Add freshness

coq/MiniML.v
@@ -1,7 +1,7 @@
 Set Implicit Arguments.
 Require Import Coq.Arith.PeanoNat Strings.String Lists.List Lia Program.Equality.
 Require Import Classes.RelationClasses Morphisms Setoid.
-Require Import CSC.Util.
+Require Import CSC.Util CSC.Fresh.
 
 Inductive bin_op :=
   | Plus
@@ -122,30 +122,39 @@ Definition of_opt_env_elem (e : option env_elem) : option val :=
 Coercion EnvAddr : addr >-> env_elem.
 Coercion EnvVal : val >-> env_elem.
 Definition Env : Set := list (string * env_elem).
-Definition State : Set := (Heap * LocMap * Env).
+Record State : Set := {
+    fresh : Fresh.fresh_state ;
+    H     : Heap ;
+    A     : LocMap;
+    Δ     : Env
+  }.
 Definition Conf : Set := (State * expr).
 
-Notation "H ';' A ';' Δ" := ((H, A, Δ) : State) (at level 80, A at next level, Δ at next level).
+Notation "F0 ';' H0 ';' A0 ';' Δ0" := ({| fresh := F0 ; H := H0 ; A := A0 ; Δ := Δ0 |} : State)
+                                  (at level 80, H0 at next level, A0 at next level, Δ0 at next level).
 Notation "Ω '▷' e" := ((Ω, e) : Conf) (at level 80, e at next level).
+Notation "∅" := ((Fresh.empty_fresh) ; (nil) ; (nil) ; (nil)).
 
-Notation "∅" := ((nil, nil, nil) : State).
+Lemma state_triv_eq Ω :
+  Ω = (Ω.(fresh); Ω.(H); Ω.(A); Ω.(Δ)).
+Proof. destruct Ω as [F H A Δ]; cbn; easy. Qed.
 
-Definition lookup {A : Type} (x : string) (Δ : list (string * A)) := Util.find (String.eqb x) Δ.
-Definition fetch (x : addr) (A : list (addr * nat)) :=
-  match Util.find (addr_eqb x) A with
+Definition Δ_lookup (x : string) (Ω : State) := Util.find (String.eqb x) Ω.(Δ).
+Definition A_lookup (x : addr) (Ω : State) :=
+  match Util.find (addr_eqb x) Ω.(A) with
   | Some n => n
   | None => 1729
   end
 .
-Definition read (a : nat) (H : list nat) :=
-  match List.nth_error H a with
+Definition H_lookup (a : nat) (Ω : State) :=
+  match List.nth_error Ω.(H) a with
   | Some n => n
   | None => 1729
   end
 .
-Lemma lookup_dec {A : Type} (x : string) (Δ : list (string * A)) :
-  { lookup x Δ = None } + { lookup x Δ <> None }.
-Proof. unfold lookup; apply Util.find_dec. Defined.
+Lemma Δ_lookup_dec (x : string) (Ω : State) :
+  { Δ_lookup x Ω = None } + { Δ_lookup x Ω <> None }.
+Proof. unfold Δ_lookup; apply Util.find_dec. Defined.
 
 Variant Event : Set :=
 | Internal : Event
@@ -166,26 +175,27 @@ Qed.
 
 Reserved Notation "Ω1 '-[' a ']~>' Ω2" (at level 80, a at next level, right associativity).
 Inductive base_step : Conf -> Event -> Conf -> Prop :=
-| VarS : forall H A Δ x v, lookup x Δ = Some (EnvVal(LitV v)) ->
-                      (H;A;Δ ▷ Var x -[ Internal ]~> H;A;Δ ▷ Lit v)
+| VarS : forall Ω x v, Δ_lookup x Ω = Some (EnvVal(LitV v)) ->
+                  (Ω ▷ Var x -[ Internal ]~> Ω ▷ Lit v)
 | BinOpS : forall Ω n1 n2 o, (Ω ▷ BinOp o (Lit n1) (Lit n2) -[ Internal ]~> Ω ▷ of_val(bin_op_eval o n1 n2))
-| GetS : forall H A Δ x n loc v nl, lookup x Δ = Some (EnvAddr loc) ->
-                               fetch loc A = nl ->
-                               read (nl + n) H = v ->
-                               (H;A;Δ ▷ Access x (Lit n) -[ Read loc n ]~> H;A;Δ ▷ Lit v)
-| SetS : forall H H' A Δ x n v loc nl, lookup x Δ = Some (EnvAddr loc) ->
-                                  fetch loc A = nl ->
-                                  H' = replace (nl + n) H v ->
-                                  (H;A;Δ ▷ Assign x (Lit n) (Lit v) -[ Write loc n ]~> H';A;Δ ▷ Lit v)
+| GetS : forall Ω x n loc v nl, Δ_lookup x Ω = Some (EnvAddr loc) ->
+                           A_lookup loc Ω = nl ->
+                           H_lookup (nl + n) Ω = v ->
+                           (Ω ▷ Access x (Lit n) -[ Read loc n ]~> Ω ▷ Lit v)
+| SetS : forall Ω H' x n v loc nl, Δ_lookup x Ω = Some (EnvAddr loc) ->
+                              A_lookup loc Ω = nl ->
+                              H' = replace (nl + n) Ω.(H) v ->
+                              (Ω ▷ Assign x (Lit n) (Lit v) -[ Write loc n ]~> Ω.(fresh);H';Ω.(A);Ω.(Δ) ▷ Lit v)
 | IfBotS : forall Ω e1 e2, (Ω ▷ If (Lit 0) e1 e2 -[ Internal ]~> Ω ▷ e2)
 | IfTopS : forall Ω e1 e2 v, v <> 0 -> (Ω ▷ If (Lit v) e1 e2 -[ Internal ]~> Ω ▷ e1)
-| LetS : forall H A Δ x v e, (H;A;Δ ▷ Letin x (Lit v) e -[ Internal ]~> H;A;((x,EnvVal (LitV v)) :: Δ) ▷ e)
-| DeleteS : forall H A Δ x loc, lookup x Δ = Some (EnvAddr loc) ->
-                           (H;A;Δ ▷ Delete x -[ Dealloc loc ]~> H;A;(delete x Δ) ▷ Lit 0)
-| NewS : forall H H' A Δ x n e loc s, s = List.length H ->
-                                 H' = grow H n ->
-                                 loc = LocA (List.length A) ->  (* <- using the length of A allows us to not need an axiom *)
-                                 (H;A;Δ ▷ New x (Lit n) e -[ Alloc loc n ]~> H';((loc, s) :: A);((x, EnvAddr loc) :: Δ) ▷ e)
+| LetS : forall Ω x v e, (Ω ▷ Letin x (Lit v) e -[ Internal ]~> Ω.(fresh);Ω.(H);Ω.(A);((x,EnvVal (LitV v)) :: Ω.(Δ)) ▷ e)
+| DeleteS : forall Ω x loc, Δ_lookup x Ω = Some (EnvAddr loc) ->
+                       (Ω ▷ Delete x -[ Dealloc loc ]~> Ω.(fresh);Ω.(H);Ω.(A);(delete x Ω.(Δ)) ▷ Lit 0)
+| NewS : forall Ω H' x n e loc s, s = List.length Ω.(H) ->
+                             H' = grow Ω.(H) n ->
+                             loc = LocA(Fresh.fresh Ω.(fresh)) ->
+                             (Ω ▷ New x (Lit n) e -[ Alloc loc n ]~>
+                                  (Fresh.advance Ω.(fresh));H';((loc, s) :: Ω.(A));((x, EnvAddr loc) :: Ω.(Δ)) ▷ e)
 where "Ω0 '-[' a ']~>' Ω1" := (base_step Ω0 a Ω1)
 .
 #[global]
@@ -265,11 +275,13 @@ Lemma fill_contextual_step Ω e1 a e2 Ω' K :
 Proof. intros H; inv H; rewrite !fill_comp; econstructor; try reflexivity; assumption. Qed.
 
 Lemma fill_steps Ω e1 As Ω' e2 K :
-  (*Ω ▷ e1 =[ As ]~>* Ω' ▷ e2 -> Ω ▷ (fill K e1) =[ As ]~>* Ω' ▷ (fill K e2).*)
-  steps (Ω ▷ e1) As (Ω' ▷ e2) -> steps (Ω ▷ (fill K e1)) As (Ω' ▷ (fill K e2)).
+  Ω ▷ e1 =[ As ]~>* Ω' ▷ e2 -> Ω ▷ (fill K e1) =[ As ]~>* Ω' ▷ (fill K e2).
 Proof.
-  intros H; dependent induction H; subst; try eapply stepsRefl.
-  eapply stepsTrans. eapply fill_contextual_step. exact H.
+  intros H.
+  pose (project := fun a : Conf => match a with | (Ω, e) => Ω ▷ fill K e end).
+  change ((fun a b => (project a) =[ As ]~>* (project b)) (Ω ▷ e1) (Ω' ▷ e2)).
+  induction H; try eapply stepsRefl.
+  eapply stepsTrans. eapply fill_contextual_step. eassumption.
   eapply IHsteps; trivial.
 Qed.
 
@@ -279,7 +291,6 @@ Ltac get_values := repeat match goal with
 Ltac context_intro := (
                        intros;
                        get_values; subst
-
                       ).
 Ltac context_solver C := (
                         match goal with
@@ -386,7 +397,7 @@ Proof. context_intro; context_solver (IfCtx HoleCtx e1 e2). Qed.
 
 Lemma contextual_step_steps σ a σ' :
   σ =[ a ]~> σ' -> σ =[ a :: nil ]~>* σ'.
-Proof. intros; destruct σ, σ'; eapply stepsTrans; (eapply stepsRefl + exact H). Qed.
+Proof. intros; destruct σ, σ'; eapply stepsTrans; (eapply stepsRefl + eassumption). Qed.
 
 #[global]
 Hint Resolve
@@ -403,30 +414,30 @@ Lemma trans_steps σ σ' σ'' As1 As2 :
 .
 Proof.
   intros H; dependent induction H; cbn; intros; try easy;
-  destruct σ''; eapply stepsTrans; try exact H; apply IHsteps; exact H1.
+  destruct σ''; eapply stepsTrans; try eassumption; apply IHsteps; eassumption.
 Qed.
 
 Lemma inv_lit_ctx_step Ω n E v Ω' :
   Ω ▷ Lit n =[ E ]~> Ω' ▷ Lit v -> Lit n = Lit v /\ Ω = Ω'.
-Proof. intros; inv H; induction K; cbn in *; try congruence; subst; inv H7. Qed.
+Proof. intros; inv H0; induction K; cbn in *; try congruence; subst; inv H8. Qed.
 
 Lemma inv_lit_steps Ω n Tr v Ω' :
   Ω ▷ Lit n =[ Tr ]~>* Ω' ▷ Lit v -> Lit n = Lit v /\ Ω = Ω' /\ Tr = nil.
 Proof.
-  intros; dependent induction H; try easy.
-  inv H; induction K; cbn in *; try congruence; subst; inv H8.
+  intros; dependent induction H0; try easy;
+  inv H0; induction K; cbn in *; try congruence; subst; inv H9.
 Qed.
 
-Lemma inv_var_ctx_step A H Δ Ω' E v s :
-  (A; H; Δ, Var s) =[ E ]~> (Ω', Lit v) -> lookup s Δ = Some(EnvVal v) /\ (A; H; Δ) = Ω'.
+Lemma inv_var_ctx_step Ω Ω' E v s :
+  (Ω, Var s) =[ E ]~> (Ω', Lit v) -> Δ_lookup s Ω = Some(EnvVal v) /\ Ω = Ω'.
 Proof. intros; inv H0; induction K; cbn in *; try congruence; subst; now inv H8. Qed.
 
-Lemma inv_var_steps A H Δ Ω' Tr v s :
-  (A; H; Δ, Var s) =[ Tr ]~>* (Ω', Lit v) -> lookup s Δ = Some(EnvVal v) /\ (A; H; Δ) = Ω' /\ Tr = Internal :: nil.
+Lemma inv_var_steps Ω Ω' Tr v s :
+  (Ω, Var s) =[ Tr ]~>* (Ω', Lit v) -> Δ_lookup s Ω = Some(EnvVal v) /\ Ω = Ω' /\ Tr = Internal :: nil.
 Proof.
   intros; dependent induction H0; try easy;
-  inv H1; induction K; cbn in *; try congruence; subst; inv H9; try easy;
-  apply inv_lit_steps in H0 as []; inv H0; now inv H1.
+  inv H0; induction K; cbn in *; try congruence; subst; inv H9; try easy;
+  apply inv_lit_steps in H1 as []; inv H1; now inv H0.
 Qed.
 
 Definition reducible (Ω : State) (e : expr) :=
@@ -455,52 +466,44 @@ Lemma closed_weaken X Y e : closed X e -> X ⊆ Y -> closed Y e.
 Proof.
   revert X Y; induction e; unfold closed; cbn; intros; eauto;
   try (rewrite bool_In_equiv_In; rewrite bool_In_equiv_In in H; now apply H0).
-  - rewrite bool_eq_equiv_if; rewrite bool_eq_equiv_if in H;
-    apply bool_and_equiv_prop; apply bool_and_equiv_prop in H;
-    destruct H; apply closed_equiv_is_closed in H, H1;
-    split; apply closed_equiv_is_closed; (eapply IHe1 + eapply IHe2); eauto.
-  - rewrite bool_eq_equiv_if; rewrite bool_eq_equiv_if in H.
-    rewrite nested_bool_pred in H; rewrite nested_bool_pred.
-    rewrite bool_and_equiv_prop in H; rewrite bool_and_equiv_prop.
-    destruct H; split.
-    + rewrite <- bool_eq_equiv_if; rewrite bool_In_equiv_In;
-      apply H0;
-      apply bool_In_equiv_In; now rewrite bool_eq_equiv_if.
-    + rewrite closed_equiv_is_closed; eapply IHe; eauto; now rewrite <- closed_equiv_is_closed.
-  - rewrite bool_eq_equiv_if; rewrite bool_eq_equiv_if in H.
-    rewrite bool_and_equiv_prop; rewrite bool_and_equiv_prop in H.
-    destruct H; split.
-    + rewrite closed_equiv_is_closed; eapply IHe1; eauto;
-      now rewrite <- closed_equiv_is_closed.
-    + rewrite closed_equiv_is_closed; eapply IHe2. instantiate (1:=s :: X).
-      now rewrite <- closed_equiv_is_closed. now apply cons_subset.
-  - rewrite bool_eq_equiv_if; rewrite bool_eq_equiv_if in H.
-    rewrite bool_and_equiv_prop; rewrite bool_and_equiv_prop in H.
-    destruct H; split.
-    + rewrite bool_and_equiv_prop; rewrite bool_and_equiv_prop in H.
-      destruct H; split.
-      * rewrite closed_equiv_is_closed; eapply IHe1; eauto; now rewrite <- closed_equiv_is_closed.
-      * rewrite closed_equiv_is_closed; eapply IHe2; eauto; now rewrite <- closed_equiv_is_closed.
-    + rewrite closed_equiv_is_closed; eapply IHe3; eauto; now rewrite <- closed_equiv_is_closed.
-  - rewrite bool_eq_equiv_if; rewrite bool_eq_equiv_if in H;
-    rewrite nested_bool_pred; rewrite nested_bool_pred in H.
-    rewrite !bool_and_equiv_prop; rewrite !bool_and_equiv_prop in H.
-    destruct H as [H []]; repeat split.
-    + rewrite <- bool_eq_equiv_if; rewrite bool_In_equiv_In;
-      apply H0;
-      apply bool_In_equiv_In; now rewrite bool_eq_equiv_if.
-    + rewrite closed_equiv_is_closed; eapply IHe1; eauto; now rewrite <- closed_equiv_is_closed.
-    + rewrite closed_equiv_is_closed; eapply IHe2; eauto; now rewrite <- closed_equiv_is_closed.
-  - rewrite bool_eq_equiv_if; rewrite bool_eq_equiv_if in H.
-    rewrite bool_and_equiv_prop; rewrite bool_and_equiv_prop in H.
-    destruct H; split.
-    + rewrite closed_equiv_is_closed; eapply IHe1; eauto;
-      now rewrite <- closed_equiv_is_closed.
-    + rewrite closed_equiv_is_closed; eapply IHe2. instantiate (1:=s :: X).
-      now rewrite <- closed_equiv_is_closed. now apply cons_subset.
+  - rewrite bool_eq_equiv_if; rewrite bool_eq_equiv_if in H0.
+    eapply subset_equiv_bool_in_subset; eassumption.
+  - rewrite bool_eq_equiv_if; rewrite bool_eq_equiv_if in H0;
+    rewrite bool_and_equiv_prop in H0; rewrite bool_and_equiv_prop;
+    destruct H0; split; rewrite <- bool_eq_equiv_if; rewrite <- bool_eq_equiv_if in H0, H2;
+    (eapply IHe1 + eapply IHe2); unfold closed; eassumption.
+  - rewrite bool_eq_equiv_if; rewrite bool_eq_equiv_if in H0;
+    apply nested_bool_pred; rewrite bool_and_equiv_prop;
+    rewrite nested_bool_pred in H0; rewrite bool_and_equiv_prop in H0;
+    split; destruct H0; try eapply subset_equiv_bool_in_subset; try eassumption;
+    rewrite <- bool_eq_equiv_if; rewrite <- bool_eq_equiv_if in H2;
+    eapply IHe; eassumption.
+  - rewrite bool_eq_equiv_if; rewrite bool_eq_equiv_if in H0;
+    rewrite bool_and_equiv_prop; rewrite bool_and_equiv_prop in H0;
+    destruct H0; split.
+    + rewrite <- bool_eq_equiv_if; rewrite <- bool_eq_equiv_if in H0; eapply IHe1; eassumption.
+    + rewrite <- bool_eq_equiv_if; rewrite <- bool_eq_equiv_if in H2; eapply IHe2; try eassumption; now apply cons_subset.
+  - rewrite bool_eq_equiv_if; rewrite bool_eq_equiv_if in H0;
+    rewrite !bool_and_equiv_prop in H0; rewrite !bool_and_equiv_prop;
+    destruct H0 as [[H2 H3] H4]; repeat split;
+    rewrite <- bool_eq_equiv_if; rewrite <- bool_eq_equiv_if in H2, H3, H4;
+    (eapply IHe1 + eapply IHe2 + eapply IHe3); eauto.
+  - rewrite bool_eq_equiv_if; rewrite bool_eq_equiv_if in H0.
+    rewrite nested_bool_pred; rewrite nested_bool_pred in H0.
+    rewrite !bool_and_equiv_prop; rewrite !bool_and_equiv_prop in H0.
+    destruct H0 as [H2 [H3 H4]]; repeat split;
+    try (eapply subset_equiv_bool_in_subset; eauto);
+    rewrite <- bool_eq_equiv_if in H3, H4;
+    rewrite <- bool_eq_equiv_if; (eapply IHe1 + eapply IHe2); eauto.
+  - rewrite bool_eq_equiv_if; rewrite bool_eq_equiv_if in H0;
+    rewrite bool_and_equiv_prop; rewrite bool_and_equiv_prop in H0;
+    destruct H0; split;
+    rewrite <- bool_eq_equiv_if; rewrite <- bool_eq_equiv_if in H0, H2;
+    (eapply IHe1 + eapply IHe2); eauto using cons_subset.
+  - erewrite bool_In_equiv_In; apply H1; apply bool_In_equiv_In in H0; assumption.
 Qed.
 Lemma closed_weaken_nil X e : closed nil e -> closed X e.
-Proof. intros; eapply closed_weaken; try exact H; intros ? ?; inv H0. Qed.
+Proof. intros; eapply closed_weaken; try exact H0; intros ? ?; inv H1. Qed.
 
 Inductive ty :=
 | tyNat : ty
@@ -509,7 +512,7 @@ Inductive ty :=
 Definition Gamma := list (string * ty).
 Reserved Notation "Γa '||-' e ':' τ '=|' Γb" (at level 99, right associativity, e at next level, τ at level 200).
 Inductive check : Gamma -> expr -> ty -> Gamma -> Prop :=
-| Tvar : forall Γ x τ, lookup x Γ = Some τ -> (Γ ||- (Var x) : τ =| Γ)
+| Tvar : forall Γ x τ, Util.find (String.eqb x) Γ = Some τ -> (Γ ||- (Var x) : τ =| Γ)
 | Tnat : forall Γ n, (Γ ||- Lit n : tyNat =| Γ)
 | Tbinop : forall Γ e1 e2 o, (Γ ||- e1 : tyNat =| Γ) ->
                         (Γ ||- e2 : tyNat =| Γ) ->
@@ -523,14 +526,14 @@ Inductive check : Gamma -> expr -> ty -> Gamma -> Prop :=
                       (Γ ||- Assign x e1 e2 : tyNat =| Γ)
 | Tlet : forall Γ Γ'' Γ''' x e1 e2, (Γ ||- e1 : tyNat =| Γ) ->
                                ((x,tyNat) :: Γ ||- e2 : tyNat =| Γ'') ->
-                               lookup x Γ'' = Some tyNat ->
+                               Util.find (String.eqb x) Γ'' = Some tyNat ->
                                Γ''' = delete x Γ'' ->
                                (Γ ||- Letin x e1 e2 : tyNat =| Γ''')
 | Tletnew : forall Γ Γ'' x e1 e2, (Γ ||- e1 : tyNat =| Γ) ->
                              ((x,tyRefnat) :: Γ ||- e2 : tyNat =| Γ'') ->
-                             lookup x Γ'' = None ->
+                             Util.find (String.eqb x) Γ'' = None ->
                              (Γ ||- New x e1 e2 : tyNat =| Γ'')
-| Tdelete : forall Γ Γ' x, lookup x Γ = Some tyRefnat ->
+| Tdelete : forall Γ Γ' x, Util.find (String.eqb x) Γ = Some tyRefnat ->
                    Γ' = delete x Γ ->
                    (Γ ||- Delete x : tyNat =| Γ')
 | Tif : forall Γ e1 e2 e3, (Γ ||- e1 : tyNat =| Γ) ->
@@ -544,9 +547,8 @@ Hint Constructors check : core.
 
 (* This is easier to work with to get traces. TODO: make it cofix when adding loops *)
 Fixpoint exec (Ω : State) (e : expr) : option (State * val * list Event) :=
-  let '(H, A, Δ) := Ω in
   match e with
-  | Var x => match lookup x Δ with
+  | Var x => match Δ_lookup x Ω with
             | Some(EnvVal(LitV v)) => Some (Ω, LitV v, Internal :: nil)
             | _ => None
             end
@@ -562,11 +564,10 @@ Fixpoint exec (Ω : State) (e : expr) : option (State * val * list Event) :=
       end
   | Access x e => match exec Ω e with
                  | Some(Ω', LitV v, Tr) =>
-                   let '(H', A', Δ') := Ω' in
-                   match lookup x Δ' with
+                   match Δ_lookup x Ω' with
                    | Some(EnvAddr loc) =>
-                       let nl := fetch loc A' in
-                       Some (Ω', LitV (read (nl + v) H'), Tr ++ ((Read loc v) :: nil))
+                       let nl := A_lookup loc Ω' in
+                       Some (Ω', LitV (H_lookup (nl + v) Ω'), Tr ++ ((Read loc v) :: nil))
                    | _ => None
                    end
                  | None => None
@@ -575,11 +576,11 @@ Fixpoint exec (Ω : State) (e : expr) : option (State * val * list Event) :=
                      | Some(Ω1, LitV n, Tr1) =>
                          match exec Ω1 e2 with
                          | Some(Ω2, LitV v, Tr2) =>
-                           let '(H', A', Δ') := Ω2 in
-                           match lookup x Δ' with
+                           match Δ_lookup x Ω2 with
                            | Some(EnvAddr loc) =>
-                               let nl := fetch loc A' in
-                               Some ((replace (nl + n) H' v, A', Δ'), LitV v, Tr1 ++ Tr2 ++ ((Write loc n)::nil))
+                               let nl := A_lookup loc Ω2 in
+                               Some ((Ω2.(fresh); replace (nl + n) Ω2.(H) v; Ω2.(A); Ω2.(Δ)),
+                                     LitV v, Tr1 ++ Tr2 ++ ((Write loc n)::nil))
                            | _ => None
                            end
                          | None => None
@@ -602,23 +603,21 @@ Fixpoint exec (Ω : State) (e : expr) : option (State * val * list Event) :=
                   end
   | Letin x e1 e2 => match exec Ω e1 with
                     | Some(Ω1, LitV v1, Tr1) =>
-                        let '(H1, A1, Δ1) := Ω1 in
-                        match exec (H1, A1, (x, EnvVal v1) :: Δ1) e2 with
+                        match exec (Ω1.(fresh); Ω1.(H); Ω1.(A); (x, EnvVal v1) :: Ω1.(Δ)) e2 with
                         | Some(Ω2, v2, Tr2) => Some(Ω2, v2, Tr1 ++ (Internal :: nil) ++ Tr2)
                         | None => None
                         end
                     | None => None
                     end
-  | Delete x => match lookup x Δ with
-               | Some (EnvAddr loc) => Some ((H, A, delete x Δ), LitV 0, (Dealloc loc)::nil)
+  | Delete x => match Δ_lookup x Ω with
+               | Some (EnvAddr loc) => Some ((Ω.(fresh); Ω.(H); Ω.(A); delete x Ω.(Δ)), LitV 0, (Dealloc loc)::nil)
                | _ => None
                end
   | New x e1 e2 => match exec Ω e1 with
                   | Some(Ω1, LitV m, Tr1) =>
-                      let '(H1, A1, Δ1) := Ω1 in
-                      let loc := LocA(List.length A1) in
-                      let s := List.length H1 in
-                      match exec (grow H1 m, (loc,s)::A1, (x,EnvAddr loc) :: Δ1) e2 with
+                      let loc := LocA(Fresh.fresh (Ω1.(fresh))) in
+                      let s := List.length (Ω1.(H)) in
+                      match exec (Fresh.advance Ω1.(fresh); grow Ω1.(H) m; (loc,s)::(Ω1.(A)); (x,EnvAddr loc) :: Ω1.(Δ)) e2 with
                       | Some(Ω2, v2, Tr2) => Some(Ω2, v2, Tr1 ++ ((Alloc loc m)::nil) ++ Tr2)
                       | _ => None
                       end
@@ -638,39 +637,35 @@ Proof. intros H; inv H; now repeat split. Qed.
 
 Ltac exec_reduce_handle_eq_none := (
   match goal with
-  | [ H1: match exec (?Aa, ?Ha, ?Δa) ?e with | Some _ => _ | None => None end = _,
-     H: exec (?Aa, ?Ha, ?Δa) ?e <> None |- _ ] =>
-      let Aa1 := fresh "Aa" in
-      let Ha1 := fresh "Ha" in
-      let Δa1 := fresh "Δa" in
+  | [ H1: match exec ?Ω ?e with | Some _ => _ | None => None end = _,
+     H: exec ?Ω ?e <> None |- _ ] =>
+      let Ωa1 := fresh "Ωa" in
       let v1 := fresh "v" in
       let Tr1 := fresh "Tr" in
-    apply Util.not_eq_None_Some in H as [x]; destruct x as [[[[Aa1 Ha1] Δa1] [v1]] Tr1];
+    apply Util.not_eq_None_Some in H as [x]; destruct x as [[Ωa1 [v1]] Tr1];
     rewrite H in H1; cbn in H1
   end;
   match goal with
-  | [Ha: (exec (?A, ?H, ?Δ) ?e = Some (?A', ?H', ?Δ', LitV ?v', ?Tr')),
+  | [Ha: (exec ?Ωa ?e = Some (?Ωa', LitV ?v', ?Tr')),
       IH: forall (Ω : State) (v : nat) (Tr : list Event) (Ω' : State),
           exec Ω ?e = Some (Ω', LitV v, Tr) ->
           (Ω, ?e) =[ Tr ]~>* (Ω', Lit v) |- _ ] =>
-      specialize (IH (A, H, Δ) v' Tr' (A', H', Δ') Ha)
+      specialize (IH Ωa v' Tr' Ωa' Ha)
   end
 ).
 
 Ltac exec_reduce := (
   try match goal with
-  | [ H: match exec (?Aa, ?Ha, ?Δa) ?e with | Some _ => _ | None => None end = _ |- _ ] =>
-      assert (exec (Aa, Ha, Δa) e <> None) by (
-      let Aa1 := fresh "Aa" in
-      let Ha1 := fresh "Ha" in
-      let Δa1 := fresh "Δa" in
+  | [ H: match exec ?Ω ?e with | Some _ => _ | None => None end = _ |- _ ] =>
+      assert (exec Ω e <> None) by (
+      let Ωa1 := fresh "Ωa" in
       let v1 := fresh "v" in
       let Tr1 := fresh "Tr" in
-      destruct (exec (Aa, Ha, Δa) e) as [[[[[Aa1 Ha1] Δa1] [v1]]]|]; congruence);
+      destruct (exec Ω e) as [[[Ωa1 [v1]]]|]; congruence);
       exec_reduce_handle_eq_none
-  | [ H: match lookup ?s ?Δa with | Some _ => _ | None => None end = _ |- _ ] =>
+  | [ H: match Δ_lookup ?s ?Ω with | Some _ => _ | None => None end = _ |- _ ] =>
     let H2 := fresh "H" in
-    destruct (lookup_dec s Δa) as [H2|H2]; try (rewrite H2 in H; congruence);
+    destruct (Δ_lookup_dec s Ω) as [H2|H2]; try (rewrite H2 in H; congruence);
     apply Util.not_eq_None_Some in H2 as [x H2];
     rewrite H2 in H; cbn in H
   | [ H: Some _ = Some _ |- _ ] => inv H
@@ -684,8 +679,8 @@ Lemma exec_is_steps Ω Ω' e v Tr :
   Ω ▷ e =[ Tr ]~>* Ω' ▷ Lit v
 .
 Proof.
-  revert Ω v Tr Ω'; induction e; intros; destruct Ω as [[Aa Ha] Δa]; cbn in H; inv H; eauto.
-  - repeat exec_reduce; destruct v0; inv H1; eauto.
+  revert Ω v Tr Ω'; induction e; intros; cbn in H0; inv H0; eauto.
+  - repeat exec_reduce; destruct v0; inv H2; eauto.
   - repeat exec_reduce;
     eapply fill_steps with (K:=LBinOpCtx b HoleCtx e2) in IHe1; cbn in IHe1;
     eapply fill_steps with (K:=RBinOpCtx b (LitV v0) HoleCtx) in IHe2; cbn in IHe2;
@@ -723,10 +718,10 @@ Lemma closed_typing Γ e τ Γ' :
   (Γ ||- e : τ =| Γ') -> closed (drop Γ) e.
 Proof.
   induction 1; subst; apply closed_equiv_is_closed; cbn.
-  - (* var *) rewrite <- bool_eq_equiv_if; erewrite bool_In_equiv_In. induction Γ; cbn. inv H.
-    destruct a. cbn in H. destruct (string_dec x s); subst.
+  - (* var *) rewrite <- bool_eq_equiv_if; erewrite bool_In_equiv_In. induction Γ; cbn in *; try congruence;
+    destruct a; cbn in *; destruct (string_dec x s); subst.
     + cbn; now left.
-    + right; apply IHΓ; apply String.eqb_neq in n; now rewrite n in H.
+    + right; apply IHΓ; apply String.eqb_neq in n; now rewrite n in H0.
   - (* lit *) easy.
   - (* binop *) apply bool_and_equiv_prop; split; apply closed_equiv_is_closed; easy.
   - (* access *) apply nested_bool_pred; apply bool_and_equiv_prop; split.
@@ -742,73 +737,70 @@ Proof.
   - (* new *) apply bool_and_equiv_prop; split.
     + rewrite <- bool_eq_equiv_if; apply closed_equiv_is_closed in IHcheck1; now apply closed_equiv_is_closed.
     + rewrite <- bool_eq_equiv_if; apply closed_equiv_is_closed in IHcheck2; now apply closed_equiv_is_closed.
-  - (* delete *) induction Γ; cbn. inv H. destruct a. cbn in H. destruct (string_dec x s); subst.
-    + cbn; destruct (string_dec s s); try contradiction; reflexivity.
-    + cbn; destruct (string_dec x s); try contradiction; apply IHΓ; apply String.eqb_neq in n; now rewrite n in H.
+  - (* delete *) induction Γ; cbn; cbn in *; try congruence. destruct a; cbn in *; destruct (string_dec x s); subst; trivial;
+    apply IHΓ; apply String.eqb_neq in n; now rewrite n in H0.
   - (* if *) rewrite !bool_and_equiv_prop; repeat split.
     + rewrite <- bool_eq_equiv_if; apply closed_equiv_is_closed in IHcheck1; now apply closed_equiv_is_closed.
     + rewrite <- bool_eq_equiv_if; apply closed_equiv_is_closed in IHcheck2; now apply closed_equiv_is_closed.
     + rewrite <- bool_eq_equiv_if; apply closed_equiv_is_closed in IHcheck3; now apply closed_equiv_is_closed.
 Qed.
 
-Lemma cons_read_same x v H :
-  read x (v :: H) = v -> read (S x) (v :: v :: H) = v.
-Proof. revert v H; induction x; intros; cbn in *; trivial. Qed.
+Lemma cons_read_same x v Ω :
+  H_lookup x (Ω.(fresh); v :: (Ω.(H)); Ω.(A); Ω.(Δ)) = v -> H_lookup (S x) (Ω.(fresh); v :: v :: (Ω.(H)); Ω.(A); Ω.(Δ)) = v.
+Proof. revert v Ω; induction x; intros; cbn in *; trivial. Qed.
 
 Lemma gprogress e τ Γ Γ' :
   (Γ ||- e : τ =| Γ') -> is_val e \/ exists Ω, reducible Ω e.
 Proof.
   induction 1; subst.
-  - (* var *) right; exists (nil, nil, (x, EnvVal(LitV 0)) :: nil); do 3 eexists; context_solver HoleCtx;
+  - (* var *) right; exists (empty_fresh; nil; nil; (x, EnvVal(LitV 0)) :: nil); do 3 eexists; context_solver HoleCtx;
     eapply VarS; cbn; now rewrite String.eqb_refl.
   - (* lit *) now left.
   - (* binop *) right; destruct (IHcheck1), (IHcheck2); get_values; subst.
     + exists ∅; do 3 eexists; context_solver HoleCtx.
-    + do 4 destruct H2 as [? H2]; do 4 eexists;
-      eapply fill_contextual_step with (K:=RBinOpCtx o (LitV x) HoleCtx) in H2; eauto.
-    + do 4 destruct H1 as [? H1]; exists x0; exists x1; exists x2;
-      exists (BinOp o x3 (Lit x)); now eapply fill_contextual_step with (K:=LBinOpCtx o HoleCtx (Lit x)) in H1.
-    + do 4 destruct H1 as [? H1]; exists x; exists x0; exists x1;
-      exists (BinOp o x2 e2); now eapply fill_contextual_step with (K:=LBinOpCtx o HoleCtx e2) in H1.
+    + do 4 destruct H1 as [? H1]; do 4 eexists;
+      eapply fill_contextual_step with (K:=RBinOpCtx o (LitV x) HoleCtx) in H1; eauto.
+    + do 4 destruct H0 as [? H0]; exists x0; exists x1; exists x2;
+      exists (BinOp o x3 (Lit x)); now eapply fill_contextual_step with (K:=LBinOpCtx o HoleCtx (Lit x)) in H0.
+    + do 4 destruct H0 as [? H0]; exists x; exists x0; exists x1;
+      exists (BinOp o x2 e2); now eapply fill_contextual_step with (K:=LBinOpCtx o HoleCtx e2) in H0.
   - (* access *) right; destruct (IHcheck2); get_values; subst.
     + do 4 eexists; context_solver HoleCtx; econstructor.
-      instantiate (1:=LocA 0); instantiate (1:=(x,EnvAddr(LocA 0))::nil); cbn; now rewrite String.eqb_refl.
-      instantiate (1:=0); instantiate (1:=(LocA 0, 0)::nil); now cbn.
-      instantiate (1:=0); instantiate (1:=grow nil (1+x0)); cbn;
-      clear IHcheck1 IHcheck2 H0. induction x0; cbn; trivial; now apply cons_read_same.
-    + do 4 destruct H1 as [? H1]; do 4 eexists;
-      eapply fill_contextual_step with (K:=AccessCtx x HoleCtx) in H1; cbn in H1; exact H1.
+      instantiate (1:=LocA 0). instantiate (1:=(empty_fresh; grow nil (1+x0); (LocA 0, 0)::nil; (x,EnvAddr(LocA 0))::nil)); cbn; now rewrite String.eqb_refl.
+      instantiate (1:=0); now cbn.
+      instantiate (1:=0); cbn; clear IHcheck1 IHcheck2 H0_0; induction x0; cbn; trivial; now apply cons_read_same.
+    + do 4 destruct H0 as [? H0]; do 4 eexists;
+      eapply fill_contextual_step with (K:=AccessCtx x HoleCtx) in H0; cbn in H0; eassumption.
   - (* assign *) right; destruct (IHcheck2), (IHcheck3); get_values; subst.
     + do 4 eexists; context_solver HoleCtx; econstructor.
-      instantiate (1:=LocA 0); instantiate (1:=(x,EnvAddr(LocA 0))::nil); cbn; now rewrite String.eqb_refl.
-      instantiate (1:=0); instantiate (1:=(LocA 0, 0)::nil); now cbn.
-      instantiate (1:=nil); instantiate (1:=nil); now destruct x1; cbn.
-    + do 4 destruct H3 as [? H3]; do 4 eexists; eapply fill_contextual_step with (K:=AssignVCtx x (LitV x0) HoleCtx) in H3; eauto.
-    + do 4 destruct H2 as [? H2]; do 4 eexists; eapply fill_contextual_step with (K:=AssignCtx x HoleCtx (Lit x0)) in H2; eauto.
-    + do 4 destruct H2 as [? H2]; do 4 eexists; eapply fill_contextual_step with (K:=AssignCtx x HoleCtx e2) in H2; eauto.
+      instantiate (1:=LocA 0). instantiate (1:=(empty_fresh; nil; (LocA 0, 0)::nil; (x, EnvAddr(LocA 0))::nil)); cbn; now rewrite String.eqb_refl.
+      instantiate (1:=0); now cbn.
+      instantiate (1:=nil); now destruct x1; cbn.
+    + do 4 destruct H1 as [? H1]; do 4 eexists; eapply fill_contextual_step with (K:=AssignVCtx x (LitV x0) HoleCtx) in H1; eauto.
+    + do 4 destruct H0 as [? H0]; do 4 eexists; eapply fill_contextual_step with (K:=AssignCtx x HoleCtx (Lit x0)) in H0; eauto.
+    + do 4 destruct H0 as [? H0]; do 4 eexists; eapply fill_contextual_step with (K:=AssignCtx x HoleCtx e2) in H0; eauto.
   - (* letin *) right; destruct (IHcheck1); get_values; subst.
-    + exists (nil, nil, nil); do 3 eexists; eauto.
-    + do 4 destruct H2 as [? H2]; do 4 eexists; eapply fill_contextual_step with (K:=LetinCtx x HoleCtx e2) in H2; eauto.
+    + exists ∅; do 3 eexists; eauto.
+    + do 4 destruct H1 as [? H1]; do 4 eexists; eapply fill_contextual_step with (K:=LetinCtx x HoleCtx e2) in H1; eauto.
   - (* new *) right; destruct (IHcheck1); get_values; subst.
-    + exists (nil, nil, nil); do 3 eexists; context_solver HoleCtx; econstructor; reflexivity.
-    + do 4 destruct H2 as [? H2]; do 4 eexists; eapply fill_contextual_step with (K:=NewCtx x HoleCtx e2) in H2; eauto.
-  - (* delete *) right; exists (nil, nil, (x,EnvAddr(LocA 0))::nil); do 3 eexists; context_solver HoleCtx;
+    + exists ∅; do 3 eexists; context_solver HoleCtx; econstructor; reflexivity.
+    + do 4 destruct H1 as [? H1]; do 4 eexists; eapply fill_contextual_step with (K:=NewCtx x HoleCtx e2) in H1; eauto.
+  - (* delete *) right; exists (empty_fresh; nil; nil; (x,EnvAddr(LocA 0))::nil); do 3 eexists; context_solver HoleCtx;
     econstructor; cbn; now rewrite String.eqb_refl.
   - (* if *) right; destruct (IHcheck1); get_values; subst.
-    + exists (nil, nil, nil); exists Internal; exists (nil, nil, nil); destruct (Nat.eq_dec x 0); subst.
+    + exists ∅; exists Internal; exists ∅; destruct (Nat.eq_dec x 0); subst.
       * exists e3; context_solver HoleCtx.
       * exists e2; context_solver HoleCtx.
-    + do 4 destruct H2 as [? H2]; eapply fill_contextual_step with (K:=IfCtx HoleCtx e2 e3) in H2; do 4 eexists; exact H2.
+    + do 4 destruct H0 as [? H0]; eapply fill_contextual_step with (K:=IfCtx HoleCtx e2 e3) in H0; do 4 eexists; eassumption.
 Qed.
 
 Lemma gprogress_steps e τ Γ Γ' :
-  (Γ ||- e : τ =| Γ') -> exists Ω Ω' Tr v, (Ω ▷ e =[ Tr ]~>* Ω' ▷ v) /\ is_val v.
+  (Γ ||- e : τ =| Γ') -> exists Ω Ω' Tr v, (Ω ▷ e =[ Tr ]~>* Ω' ▷ v) \/ is_val v.
 Proof.
-  intros; apply gprogress in H as [].
-  - do 2 exists ∅. exists nil. apply is_val_inv in H as []. exists (Lit x). subst. repeat constructor.
-  - destruct H as [Ω [E [Ω' [e' H]]]]. exists Ω. exists Ω'. exists (E :: nil). exists e'. split. eapply stepsTrans. exact H. eapply stepsRefl.
-    (* Logical Relations .... *)
-Admitted.
+  intros; apply gprogress in H0 as [].
+  - do 2 exists ∅; exists nil; apply is_val_inv in H0 as []; exists (Lit x); subst; repeat constructor.
+  - destruct H0 as [Ω [E [Ω' [e' H0]]]]; exists Ω; exists Ω'; exists (E :: nil); exists e'; left; eapply stepsTrans; try eassumption; eapply stepsRefl.
+Qed.
 
 Lemma preservation e e' Γ Γ' Ω Ω' a :
   (Γ ||- e : tyNat =| Γ') ->
@@ -818,25 +810,23 @@ Lemma preservation e e' Γ Γ' Ω Ω' a :
 Proof.
 Admitted.
 
-Axiom zap : forall e : expr, exists Ω E Ω' v, Ω ▷ e =[ E ]~> Ω' ▷ Lit v.
-
 Lemma binop_ctx_step_inv Ω1 b e1 e2 Ω3 v E :
   Ω1 ▷ BinOp b e1 e2 =[ E ]~> Ω3 ▷ Lit v ->
   exists v1 v2, (e1 = Lit v1 /\ e2 = Lit v2 /\ E = Internal /\ v = bin_op_eval_int b v1 v2)
 .
 Proof.
-  intros. inv H. induction K; cbn in *; try congruence. subst.
-  inv H7. exists n1; exists n2; easy.
+  intros; inv H0; induction K; cbn in *; try congruence; subst;
+  inv H8; exists n1; exists n2; easy.
 Qed.
 
 Lemma binop_steps_lits_inv Ω1 b Ω3 v1 v2 v Tr :
   Ω1 ▷ BinOp b (Lit v1) (Lit v2) =[ Tr ]~>* Ω3 ▷ Lit v ->
   Ω1 = Ω3 /\ v = v1 + v2 /\ Tr = Internal :: nil.
 Proof.
-  intros; inv H; inv H4; destruct K; cbn in *; try congruence; subst.
-  - inv H8; apply inv_lit_steps in H6 as [H [H0 H1]]; subst; inv H; easy.
-  - inv H5; destruct K; cbn in *; try congruence; subst; inv H8.
-  - inv H5; destruct K; cbn in *; try congruence; subst; inv H8.
+  intros; inv H0; inv H5; destruct K; cbn in *; try congruence; subst.
+  - inv H9; apply inv_lit_steps in H7 as [H [H0 H1]]; subst; inv H; easy.
+  - inv H6; destruct K; cbn in *; try congruence; subst; inv H9.
+  - inv H6; destruct K; cbn in *; try congruence; subst; inv H9.
 Qed.
 
 Lemma binop_steps_inv Ω1 b e1 e2 Ω3 v Tr :
@@ -847,20 +837,19 @@ Lemma binop_steps_inv Ω1 b e1 e2 Ω3 v Tr :
 Proof.
 Admitted.
 
-Lemma access_steps_inv Ω1 A3 H3 Δ3 s e v Tr :
-  Ω1 ▷ Access s e =[ Tr ]~>* (H3; A3; Δ3) ▷ Lit v ->
+Lemma access_steps_inv Ω1 Ω3 s e v Tr :
+  Ω1 ▷ Access s e =[ Tr ]~>* Ω3 ▷ Lit v ->
   exists Ω' Tr' loc v1, ((Ω1 ▷ e =[ Tr' ]~>* Ω' ▷ Lit v1)
-/\ (let '(H', A', Δ') := Ω' in (A3 = A' /\ H3 = H' /\ Δ3 = Δ' /\ v = read (fetch loc A' + v1) H')
-/\ lookup s Δ' = Some(EnvAddr loc) /\ Tr = Tr' ++ Read loc v1 :: nil))
+/\ (Ω3 = Ω' /\ v = H_lookup (A_lookup loc Ω' + v1) Ω')
+/\ Δ_lookup s Ω' = Some(EnvAddr loc) /\ Tr = Tr' ++ Read loc v1 :: nil)
 .
 Proof.
-  intros. dependent induction H.
 Admitted.
 
 Lemma letin_steps_inv Ω1 Ω3 s e1 e2 v Tr :
   Ω1 ▷ Letin s e1 e2 =[ Tr ]~>* Ω3 ▷ Lit v ->
-  exists H1 A1 Δ1 Tr1 Tr2 v1 v2, (Ω1 ▷ e1 =[ Tr1 ]~>* (H1; A1; Δ1) ▷ Lit v1)
-/\ ((H1; A1; (s,EnvVal v1) :: Δ1) ▷ e2 =[ Tr2 ]~>* Ω3 ▷ Lit v2) /\ v = v2 /\ Tr = Tr1 ++ Internal :: Tr2
+  exists Ω2 Tr1 Tr2 v1 v2, (Ω1 ▷ e1 =[ Tr1 ]~>* Ω2 ▷ Lit v1)
+/\ ((Ω2.(fresh); Ω2.(H); Ω2.(A); (s,EnvVal v1) :: Ω2.(Δ)) ▷ e2 =[ Tr2 ]~>* Ω3 ▷ Lit v2) /\ v = v2 /\ Tr = Tr1 ++ Internal :: Tr2
 .
 Proof.
 Admitted.
@@ -875,12 +864,12 @@ Lemma if_steps_inv Ω Ω' e1 e2 e3 v Tr :
 Proof.
 Admitted.
 
-Lemma assign_steps_inv Ω H' A' Δ' s e1 e2 v Tr :
-  Ω ▷ Assign s e1 e2 =[ Tr ]~>* (H'; A'; Δ') ▷ Lit v ->
+Lemma assign_steps_inv Ω Ω' s e1 e2 v Tr :
+  Ω ▷ Assign s e1 e2 =[ Tr ]~>* Ω' ▷ Lit v ->
   exists v1 Tr1 Ω1 v2 Tr2 Ω2 loc, (Ω ▷ e1 =[ Tr1 ]~>* Ω1 ▷ Lit v1) /\ (Ω1 ▷ e2 =[ Tr2 ]~>* Ω2 ▷ Lit v2)
-/\ (let '(H2, A2, Δ2) := Ω2 in (lookup s Δ2 = Some(EnvAddr loc)
-                             /\ Tr = Tr1 ++ Tr2 ++ Write loc v1 :: nil /\ v = v2
-                             /\ H' = replace (fetch loc A' + v1) H2 v2 /\ A' = A2 /\ Δ' = Δ2))
+/\ ((Δ_lookup s Ω2 = Some(EnvAddr loc)
+                             /\ Tr = Tr1 ++ Tr2 ++ Write loc v1 :: nil /\ v = v2 /\ Ω'.(fresh) = Ω2.(fresh)
+                             /\ Ω'.(H) = replace (A_lookup loc Ω2 + v1) Ω2.(H) v2 /\ Ω'.(A) = Ω2.(A) /\ Ω'.(Δ) = Ω2.(Δ)))
 .
 Proof.
 Admitted.
@@ -888,23 +877,24 @@ Admitted.
 Lemma new_steps_inv Ω Ω' s e1 e2 v Tr :
   Ω ▷ New s e1 e2 =[ Tr ]~>* Ω' ▷ Lit v ->
   exists v1 Tr1 Ω1 v2 Tr2 Ω2, (Ω ▷ e1 =[ Tr1 ]~>* Ω1 ▷ Lit v1)
-/\ (let '(H1, A1, Δ1) := Ω1 in (((grow H1 v1; (LocA(List.length A1), List.length H1) :: A1; (s,EnvAddr(LocA(List.length A1))) :: Δ1)
+/\ (((Fresh.advance (Ω1.(fresh)); grow Ω1.(H) v1;
+     (LocA(Fresh.fresh Ω1.(fresh)), List.length Ω1.(H)) :: (Ω1.(A)); (s,EnvAddr(LocA(Fresh.fresh (Ω1.(fresh))))) :: (Ω1.(Δ))
                                 ▷ e2 =[ Tr2 ]~>* Ω2 ▷ Lit v2)
-/\  Ω' = Ω2 /\ v = v2 /\ Tr = Tr1 ++ Alloc (LocA(List.length A1)) v1 :: Tr2))
+/\  Ω' = Ω2 /\ v = v2 /\ Tr = Tr1 ++ Alloc (LocA(Fresh.fresh(Ω1.(fresh)))) v1 :: Tr2))
 .
 Proof.
 Admitted.
 
 Lemma delete_steps_inv Ω Ω' s Tr v :
   Ω ▷ Delete s =[ Tr ]~>* Ω' ▷ Lit v ->
-  exists loc, (let '(Ha, Aa, Δa) := Ω in (lookup s Δa = Some(EnvAddr loc)
-      /\ Ω' = (Ha, Aa, delete s Δa) /\ v = 0 /\ Tr = Dealloc loc :: nil
-  )).
+  exists loc, (Δ_lookup s Ω = Some(EnvAddr loc)
+      /\ Ω' = (Ω.(fresh); Ω.(H); Ω.(A); delete s Ω.(Δ)) /\ v = 0 /\ Tr = Dealloc loc :: nil
+  ).
 Proof.
-  intros; destruct Ω; inv H;
-  inv H4; induction K; cbn in *; try congruence; subst; inv H8;
-  exists loc; repeat split; apply inv_lit_steps in H6 as [H0 [H1 H2]]; try easy;
-  now (inv H0 + rewrite H2).
+  intros; destruct Ω; inv H0.
+  inv H6; induction K; cbn in *; try congruence; subst; inv H10;
+  exists loc; repeat split; apply inv_lit_steps in H8 as [Hx0 [Hx1 Hx2]]; try easy;
+  now (inv Hx0 + rewrite Hx2).
 Qed.
 
 (* this depends on the above inversion lemmas... *)
@@ -913,34 +903,36 @@ Lemma steps_is_exec Ω Ω' e v Tr :
   exec Ω e = Some (Ω', LitV v, Tr)
 .
 Proof.
-  revert Ω v Tr Ω'; induction e; intros; destruct Ω as [[Ha Aa] Δa], Ω' as [[Ha' Aa'] Δa']; cbn.
-  - apply inv_lit_steps in H as []; subst; inv H0; inv H; inv H1; easy.
-  - apply inv_var_steps in H as [H []]; rewrite H, H1; inv H0; easy.
-  - eapply binop_steps_inv in H as [Ω2 [Tr1 [Tr2 [v1 [v2 [H1 [H2 [H3 H4]]]]]]]];
-    specialize (IHe1 (Ha; Aa; Δa) v1 Tr1 Ω2 H1); specialize (IHe2 Ω2 v2 Tr2 (Ha'; Aa'; Δa') H2);
+  revert Ω v Tr Ω'; induction e; intros; cbn.
+  - apply inv_lit_steps in H0 as []; subst; inv H1; inv H0; easy.
+  - apply inv_var_steps in H0 as [H0 []]; now rewrite H0, H1, H2.
+  - eapply binop_steps_inv in H0 as [Ω2 [Tr1 [Tr2 [v1 [v2 [H1 [H2 [H3 H4]]]]]]]];
+    specialize (IHe1 Ω v1 Tr1 Ω2 H1); specialize (IHe2 Ω2 v2 Tr2 Ω' H2);
     now rewrite IHe1, IHe2, H3, H4.
-  - eapply access_steps_inv in H as [[[H' A'] Δ'] [Tr' [loc [v1 [H1 [[H2 [H3 [H4 H5]]] [H6 H7]]]]]]];
-    specialize (IHe (Ha; Aa; Δa) v1 Tr' (H'; A'; Δ') H1);
-    now rewrite IHe, H6, H5, H7, H2, H3, H4.
-  - eapply letin_steps_inv in H as [H1 [A1 [Δ1 [Tr1 [Tr2 [v1 [v2 [H2 [H3 [H4 H5]]]]]]]]]];
-    specialize (IHe1 (Ha; Aa; Δa) v1 Tr1 (H1; A1; Δ1) H2);
-    specialize (IHe2 (H1; A1; (s, EnvVal v1) :: Δ1) v2 Tr2 (Ha'; Aa'; Δa') H3);
+  - eapply access_steps_inv in H0 as [Ω0 [Tr' [loc [v1 [H0 [[H1 H2] [H3 H4]]]]]]];
+    specialize (IHe Ω v1 Tr' Ω0 H0);
+    now rewrite IHe, H1, H2, H3, H4.
+  - eapply letin_steps_inv in H0 as [Ω1 [Tr1 [Tr2 [v1 [v2 [H2 [H3 [H4 H5]]]]]]]].
+    specialize (IHe1 Ω v1 Tr1 Ω1 H2);
+    specialize (IHe2 (Ω1.(fresh); Ω1.(H); Ω1.(A); (s, EnvVal v1) :: Ω1.(Δ)) v2 Tr2 Ω' H3);
     now rewrite IHe1, IHe2, H4, H5.
-  - eapply if_steps_inv in H as [v1 [Tr1 [Ω1 [H1 [[H2 [v2 [Tr2 [Ω2 [H3 [H4 [H5 H6]]]]]]]
-                                                | [H2 [v3 [Tr3 [Ω3 [H3 [H4 [H5 H6]]]]]]]]]]]];
-    specialize (IHe1 (Ha; Aa; Δa) v1 Tr1 Ω1 H1).
+  - eapply if_steps_inv in H0 as [v1 [Tr1 [Ω1 [H1 [[H2 [v2 [Tr2 [Ω2 [H3 [H4 [H5 H6]]]]]]]
+                                                 | [H2 [v3 [Tr3 [Ω3 [H3 [H4 [H5 H6]]]]]]]]]]]];
+    specialize (IHe1 Ω v1 Tr1 Ω1 H1).
     + specialize (IHe2 Ω1 v2 Tr2 Ω2 H3);
       destruct v1; try contradiction; now rewrite IHe1, IHe2, H4, H5, H6.
     + specialize (IHe3 Ω1 v3 Tr3 Ω3 H3);
       now rewrite IHe1, IHe3, H4, H2, H5, H6.
-  - eapply assign_steps_inv in H as [v1 [Tr1 [Ω1 [v2 [Tr2 [[[H2 A2] Δ2] [loc [H3 [H4 [H5 [H6 [H7 [H8 [H9 H10]]]]]]]]]]]]]];
-    specialize (IHe1 (Ha; Aa; Δa) v1 Tr1 Ω1 H3); specialize (IHe2 Ω1 v2 Tr2 (H2; A2; Δ2) H4);
-    now rewrite IHe1, IHe2, H5, H6, H7, H8, H9, H10.
-  - eapply new_steps_inv in H as [v1 [Tr1 [[[H1 A1] Δ1] [v2 [Tr2 [Ω2 [H2 [H3 [H4 [H5 H6]]]]]]]]]];
-    specialize (IHe1 (Ha; Aa; Δa) v1 Tr1 (H1; A1; Δ1) H2);
-    specialize (IHe2 (grow H1 v1; (LocA(List.length A1), List.length H1) :: A1; (s, EnvAddr(LocA(List.length A1))) :: Δ1) v2 Tr2 Ω2 H3);
+  - eapply assign_steps_inv in H0 as [v1 [Tr1 [Ω1 [v2 [Tr2 [Ω2 [loc [H3 [H4 [H5 [H6 [H7 [H8 [H9 [H10 H11]]]]]]]]]]]]]]].
+    specialize (IHe1 Ω v1 Tr1 Ω1 H3); specialize (IHe2 Ω1 v2 Tr2 Ω2 H4);
+    rewrite IHe1, IHe2, H5, H6, H7, <- H8, <- H9, <- H10, <- H11; repeat f_equal; destruct Ω'; now cbn.
+  - eapply new_steps_inv in H0 as [v1 [Tr1 [Ω1 [v2 [Tr2 [Ω2 [H2 [H3 [H4 [H5 H6]]]]]]]]]];
+    specialize (IHe1 Ω v1 Tr1 Ω1 H2);
+    specialize (IHe2 (advance (Ω1.(fresh)); grow Ω1.(H) v1;
+                      (LocA(Fresh.fresh (Ω1.(fresh))), List.length Ω1.(H)) :: (Ω1.(A));
+                      (s, EnvAddr(LocA(Fresh.fresh (Ω1.(fresh))))) :: Ω1.(Δ)) v2 Tr2 Ω2 H3);
     now rewrite IHe1, IHe2, H4, H5, H6.
-  - eapply delete_steps_inv in H as [loc [H1 [H2 [H3 H4]]]];
+  - eapply delete_steps_inv in H0 as [loc [H1 [H2 [H3 H4]]]];
     now rewrite H1, H2, H3, H4.
 Qed.
 
@@ -1043,21 +1035,21 @@ Lemma temp_memsafe_is_safety : safety temp_memsafe.
 Proof.
   intros ? ?.
   exists (Dealloc (LocA 0) :: Read (LocA 0) 42 :: nil); intros ? ? ? ?.
-  unfold temp_memsafe in H, H2.
-  eapply H2. exact 5.  (* <- this makes it seem like something is off of the definition *)
+  unfold temp_memsafe in H0, H3.
+  eapply H3. exact 5.  (* <- this makes it seem like something is off of the definition *)
   intros ?. exists 0. intros. exists 1. split; try lia.
   (* by prefix *)
 Admitted.
 Lemma spat_memsafe_is_safety : safety spat_memsafe.
 Proof.
-  intros ? ?.
-  exists (Alloc (LocA 0) 42 :: Read (LocA 0) 1337 :: nil); intros ? ? ? ?.
-  eapply prefix_implies_occ with (e:=Alloc (LocA 0) 42) in H1 as Halloc1; cbn; try now left.
-  eapply prefix_implies_occ with (e:=Read (LocA 0) 1337) in H1 as Hread1; cbn; try (right; now left).
-  specialize (H2 (LocA 0) 42 Halloc1) as [].
-  assert (occ (Read (LocA 0) 1337) t') by assumption.
+  intros t H0.
+  exists (Alloc (LocA 0) 42 :: Read (LocA 0) 1337 :: nil); intros H2 t' H3 H4.
+  eapply prefix_implies_occ with (e:=Alloc (LocA 0) 42) in H3 as Halloc1; cbn; try now left.
+  eapply prefix_implies_occ with (e:=Read (LocA 0) 1337) in H3 as Hread1; cbn; try (right; now left).
+  specialize (H4 (LocA 0) 42 Halloc1) as [].
+  assert (occ (Read (LocA 0) 1337) t') as H5 by assumption.
   destruct Hread1 as [n1 Hread1'].
-  specialize (H2 1337 H4).
+  specialize (H1 1337 H5).
   lia.
 Qed.
 
@@ -1065,7 +1057,7 @@ Lemma plug_checks_propagate (c : WhileContext) (p : WhileComponent) :
   context_check c ->
   component_check p ->
   whole_program_check (plug c p).
-Proof. intros; destruct c, H, H0; cbn; repeat (econstructor; trivial); (eassumption || now cbn). Defined.
+Proof. intros H H0; destruct c, H, H0; cbn; repeat (econstructor; trivial); (eassumption || now cbn). Defined.
 
 Definition termtrace : CTrace.
 Proof.
@@ -1123,8 +1115,4 @@ Lemma while_is_temp_memsafe (p : WhileComponent) (H : component_check p) :
   wrsat H temp_memsafe.
 Proof.
   destruct p; destruct H as [e' HΓ].
-  intros ? ? ? ? ?; split; remember (plug c0 (WComp e' (closed_typing HΓ))) as fp; destruct fp.
-  - destruct H as [n [Ha Hb]].
-
-    induction e0; cbn in *; try now apply alloc_not_in_termtrace in Ha.
 Admitted.
