coq/Fresh.v
@@ -1,0 +1,8 @@
+Set Implicit Arguments.
+
+Record fresh_state := { counter : nat }.
+
+Definition empty_fresh := {| counter := 0 |}.
+Definition fresh (x : fresh_state) : nat := x.(counter).
+Definition advance (x : fresh_state) : fresh_state := {| counter := x.(counter) + 1 |}.
+
